Intermediate/GlobalEnv.v
@@ -11,6 +11,25 @@ Record global_env := mkGlobalEnv {
   genv_entrypoints : EntryPoint.t;
 }.
 
+Record well_formed_global_env (G: global_env) := {
+  wfgenv_interface_soundness:
+    sound_interface (genv_interface G);
+  wfgenv_entrypoints_soundness:
+    forall C, NMap.In C (genv_entrypoints G) -> NMap.In C (genv_interface G);
+  wfgenv_procedures_soundness:
+    forall C, NMap.In C (genv_procedures G) -> NMap.In C (genv_interface G)
+}.
+
+(* G contains G', moreover they share the same interface *)
+Definition genv_extension (G G': global_env) : Prop :=
+  NMap.Equal (genv_interface G) (genv_interface G') /\
+  forall C, (forall Cprocs,
+           NMap.MapsTo C Cprocs (genv_procedures G') ->
+           NMap.MapsTo C Cprocs (genv_procedures G)) /\
+       (forall Centrypoints,
+           NMap.MapsTo C Centrypoints (genv_entrypoints G') ->
+           NMap.MapsTo C Centrypoints (genv_entrypoints G)).
+
 Definition executing G (pc : Pointer.t) (i : instr) : Prop :=
   exists C_procs P_code,
     NMap.find (Pointer.component pc) (genv_procedures G) = Some C_procs /\
@@ -66,3 +85,9 @@ Definition init_genv (p: program) : global_env :=
   {| genv_interface := prog_interface p;
      genv_procedures := ps;
      genv_entrypoints := E |}.
+
+Lemma init_genv_preserves_well_formedness:
+  forall p, well_formed_program p ->
+       well_formed_global_env (init_genv p).
+Proof.
+Admitted.
