Intermediate/PS.v
@@ -25,6 +25,11 @@ Inductive state : Type :=
 | CC : context_state -> exec_state -> state
 with exec_state : Type := Normal | WentWrong.
 
+(* The split between program and context is represented by the domain of the
+   entrypoints map. *)
+Definition is_program_component G C := NMap.In C (genv_entrypoints G).
+Definition is_context_component G C := ~ is_program_component G C.
+
 Definition initial_state
            (G: global_env)
            (mainC: Component.id) (mainP: Procedure.id)
@@ -36,14 +41,18 @@ Definition initial_state
     (* the program counter is pointing to the start of the main procedure *)
     EntryPoint.get mainC mainP (genv_entrypoints G) = Some (Pointer.block pc) /\
     Pointer.component pc = mainC /\
-    Pointer.offset pc = 0
+    Pointer.offset pc = 0 /\
+    (* each program component has its own memory *)
+    (forall C, is_program_component G C -> NMap.In C mem)
   | CC (pgps, mem, C) execst =>
     (* the global protected stack is empty *)
     pgps = [] /\
     (* the execution didn't go wrong *)
     execst = Normal /\
     (* the executing component is the main one *)
-    C = mainC
+    C = mainC /\
+    (* each program component has its own memory *)
+    (forall C, is_program_component G C -> NMap.In C mem)
   end.
 
 Definition final_state (G: global_env) (s: state) (r: nat) : Prop :=
@@ -62,7 +71,7 @@ Definition to_partial_frame pc frame : PartialPointer.t :=
 Definition to_partial_stack (s : CS.stack) (pc : list Component.id) :=
   map (to_partial_frame pc) s.
 
-Lemma push_by_prog_preserves_partial_stack :
+Lemma push_by_prog_preserves_partial_stack:
   forall s ps pc C b o,
     Util.Lists.mem C pc = true ->
     to_partial_stack s pc = ps ->
@@ -72,7 +81,7 @@ Proof.
   simpl. rewrite Hprogturn. rewrite H. reflexivity.
 Qed.
 
-Lemma push_by_context_preserves_partial_stack :
+Lemma push_by_context_preserves_partial_stack:
   forall s ps pc C b o,
     ~ (In C pc) ->
     to_partial_stack s pc = ps ->
@@ -83,22 +92,25 @@ Proof.
   rewrite Hprogturn. rewrite Hpstack. reflexivity.
 Qed.
 
-(* The split between program and context is represented by the domain of the
-   entrypoints map. *)
-Definition is_program_component G C := NMap.In C (genv_entrypoints G).
-Definition is_context_component G C := ~ is_program_component G C.
-
 Inductive step (G : global_env) : state -> trace -> state -> Prop :=
 | Program_Epsilon:
-    forall gps pgps
-      (mem mem' wmem wmem' : Memory.t) cmem cmem'
+    forall G' pgps (mem mem' wmem wmem' : Memory.t) Cmem'
       (regs regs' : Register.t) (pc pc' : Pointer.t),
-      let C := Pointer.component pc in
-      NMap.MapsTo C cmem wmem ->
-      NMap.MapsTo C cmem' wmem' ->
-      CS.step G (gps,wmem,regs,pc) E0 (gps,wmem',regs',pc') ->
-      NMap.MapsTo C cmem mem ->
-      NMap.MapsTo C cmem' mem' ->
+      (* G' has the same interface as G, but it can contain more
+         information regarding procedures and entrypoints *)
+      genv_extension G' G ->
+      (* wmem contains mem *)
+      (forall C Cmem, NMap.MapsTo C Cmem mem -> NMap.MapsTo C Cmem wmem) ->
+      (* wmem has the context components memories *)
+      (forall C, is_context_component G C -> NMap.In C wmem) ->
+      (* the complete semantics steps silently with the extended versions of
+         memory and global environment
+         NOTE that the stack (gps) is not related to the partial one (pgps) *)
+      (exists gps, CS.step G' (gps,wmem,regs,pc) E0 (gps,wmem',regs',pc')) ->
+      (* mem' is mem with the updated version of the current
+         executing component's memory *)
+      NMap.MapsTo (Pointer.component pc) Cmem' wmem' ->
+      NMap.Equal mem' (NMap.add (Pointer.component pc) Cmem' mem) ->
       step G (PC (pgps,mem,regs,pc)) E0 (PC (pgps,mem',regs',pc'))
 
 | Program_Internal_Call:
@@ -113,7 +125,7 @@ Inductive step (G : global_env) : state -> trace -> state -> Prop :=
       Register.get R_COM regs = Int val ->
       let pc' := (C', b, 0) in
       let t := [ECall C P val C'] in
-      step G (PC (pgps,mem,regs,pc)) t (PC (pgps',mem,regs,pc'))
+      step G (PC (pgps,mem,regs,pc)) t (PC (pgps',mem,Register.invalidate regs,pc'))
 
 | Program_Internal_Return:
     forall pgps pgps' mem regs pc pc' C' b o val,
@@ -124,7 +136,7 @@ Inductive step (G : global_env) : state -> trace -> state -> Prop :=
       is_program_component G C' ->
       Register.get R_COM regs = Int val ->
       let t := [ERet C val C'] in
-      step G (PC (pgps,mem,regs,pc)) t (PC (pgps',mem,regs,pc'))
+      step G (PC (pgps,mem,regs,pc)) t (PC (pgps',mem,Register.invalidate regs,pc'))
 
 | Program_External_Call:
     forall pgps pgps' mem regs pc C' b o P val,
@@ -195,24 +207,28 @@ Inductive step (G : global_env) : state -> trace -> state -> Prop :=
       let t := [ERet C val C'] in
       step G (CC (pgps,mem,C) Normal) t (PC (pgps',mem,regs, (C',b,o))).
 
-Definition partialize (p: program) (ctx: Program.interface) : program :=
-  {| prog_interface := prog_interface p;
-     prog_procedures :=
-       NMapExtra.filter (fun C _ => negb (NMap.mem C ctx)) (prog_procedures p);
-     prog_buffers :=
-       NMapExtra.filter (fun C _ => negb (NMap.mem C ctx)) (prog_buffers p);
-     prog_main := prog_main p |}.
+Definition partialize (p: program) (ctx: Program.interface)
+           (mainC: Component.id) (mainP: Procedure.id)
+  : program :=
+  {| prog_interface := NMapExtra.update (prog_interface p) ctx;
+     prog_procedures := prog_procedures p;
+     prog_buffers := prog_buffers p;
+     prog_main := (mainC, mainP) |}.
 
 Section Semantics.
   Variable p: program.
+  Variable mainC: Component.id.
+  Variable mainP: Procedure.id.
   Variable context_interface : Program.interface.
 
-  Definition partial_program := partialize p context_interface.
+  Definition partial_program := partialize p context_interface mainC mainP.
+
   Let G := init_genv partial_program.
 
   Definition sem :=
     @Semantics_gen state global_env step
-                   (initial_state G (fst (prog_main p)) (snd (prog_main p)))
+                   (initial_state G (fst (prog_main partial_program))
+                                    (snd (prog_main partial_program)))
                    (final_state G) G.
 End Semantics.
 
