Source/GlobalEnv.v
@@ -1,5 +1,6 @@
 Require Import Common.Definitions.
 Require Import Common.Values.
+Require Import Common.Linking.
 Require Import Source.Language.
 
 Import Source.
@@ -9,6 +10,25 @@ Record global_env : Type := mkGlobalEnv {
   genv_procedures : NMap.t (NMap.t expr);
   genv_buffers : NMap.t Block.id
 }.
+
+Record well_formed_global_env (G: global_env) := {
+  wfgenv_interface_soundness:
+    sound_interface (genv_interface G);
+  wfgenv_procedures_soundness:
+    forall C, NMap.In C (genv_procedures G) -> NMap.In C (genv_interface G);
+  wfgenv_buffers_soundness:
+    forall C, NMap.In C (genv_buffers G) -> NMap.In C (genv_interface G)
+}.
+
+(* G contains G', moreover they share the same interface *)
+Definition genv_extension (G G': global_env) : Prop :=
+  NMap.Equal (genv_interface G) (genv_interface G') /\
+  forall C, (forall Cprocs,
+           NMap.MapsTo C Cprocs (genv_procedures G') ->
+           NMap.MapsTo C Cprocs (genv_procedures G)) /\
+       (forall Cbufs,
+           NMap.MapsTo C Cbufs (genv_buffers G') ->
+           NMap.MapsTo C Cbufs (genv_buffers G)).
 
 Definition init_genv (p: program) : global_env :=
   let '(bufs, _) := init_all p in
