Intermediate/Decomposition.v
@@ -13,18 +13,49 @@ Import Intermediate.
 
 Section Decomposition.
   Variables p c: program.
+  Variable mainC: Component.id.
+  Variable mainP: Procedure.id.
 
-  Let mainC := fst (prog_main p).
-  Let mainP := snd (prog_main p).
+  (* p and c are valid programs *)
+  Hypothesis pWF: well_formed_program p.
+  Hypothesis cWF: well_formed_program c.
+
+  (* linking p and c results in a valid closed program *)
+  (* (we assume to have a valid main procedure from which to start execution) *)
+  (* partializing still return a partial program *)
+  Hypothesis pcWF:
+    well_formed_program (program_link p c mainC mainP).
+  Hypothesis pcClosed:
+    closed_program (program_link p c mainC mainP).
+  Hypothesis partialWF:
+    well_formed_program (PS.partial_program p mainC mainP (prog_interface c)).
+
   Let split := map fst (NMap.elements (prog_interface p)).
-  Let G := init_genv (program_link p c (prog_main p)).
-  Let G' := init_genv (PS.partial_program p (prog_interface c)).
+  Let G := init_genv (program_link p c mainC mainP).
+  Let G' := init_genv (PS.partial_program p mainC mainP (prog_interface c)).
+
+  Lemma G_is_well_formed:
+    well_formed_global_env G.
+  Proof.
+    apply (init_genv_preserves_well_formedness
+             (program_link p c mainC mainP));
+      auto.
+  Qed.
+
+  Lemma G'_is_well_formed:
+    well_formed_global_env G'.
+  Proof.
+    apply (init_genv_preserves_well_formedness
+             (PS.partial_program p mainC mainP (prog_interface c)));
+      auto.
+  Qed.
 
   Inductive related_states : CS.state -> PS.state -> Prop :=
   | ProgramControl:
       forall gps pgps mem pmem regs pc,
         PS.is_program_component G (Pointer.component pc) ->
         pgps = PS.to_partial_stack gps split ->
+        NMap.In (Pointer.component pc) mem ->
         PS.maps_match_on split mem pmem ->
         related_states (gps, mem, regs, pc)
                        (PS.PC (pgps, pmem, regs, pc))
@@ -32,6 +63,7 @@ Section Decomposition.
       forall gps pgps mem pmem regs pc,
         PS.is_context_component G (Pointer.component pc) ->
         pgps = PS.to_partial_stack gps split ->
+        NMap.In (Pointer.component pc) mem ->
         PS.maps_match_on split mem pmem ->
         related_states (gps, mem, regs, pc)
                        (PS.CC (pgps, pmem, Pointer.component pc) PS.Normal)
@@ -39,6 +71,7 @@ Section Decomposition.
       forall gps pgps mem pmem regs pc,
         PS.is_context_component G (Pointer.component pc) ->
         pgps = PS.to_partial_stack gps split ->
+        NMap.In (Pointer.component pc) mem ->
         PS.maps_match_on split mem pmem ->
         (forall s' t, ~ CS.step G (gps,mem,regs,pc) t s') ->
         ~ (forall r, CS.final_state G (gps,mem,regs,pc) r) ->
@@ -53,30 +86,32 @@ Section Decomposition.
   Proof.
     intros s1 Hs1_init.
     CS.unfold_state.
-    destruct Hs1_init as [Hempty_stack [Hpc_comp [Hpc_block Hpc_offset]]].
+    destruct Hs1_init as [Hempty_stack [[Hpc_comp [Hpc_block Hpc_offset]] Hmem]].
     destruct (NMapExtra.F.In_dec (genv_entrypoints G) mainC) as [Hprg|Hctx].
     - exists (PS.PC (PS.to_partial_stack s split, mem, regs, pc)).
       split.
       + unfold PS.initial_state.
         subst. repeat split; eauto.
-        unfold G'.
-        (* TODO prove linking doesn't create problems *)
-        admit.
+        unfold G, G'.
+        * admit. (* TODO prove that entrypoints are the same in both G and G' *)
+        * admit. (* TODO prove that program components have a memory *)
       + apply ProgramControl; auto.
         * unfold PS.is_program_component.
-          subst mainC. rewrite Hpc_comp.
-          auto.
+          subst mainC. auto.
+        * apply Hmem. rewrite Hpc_comp.
+          apply wfgenv_entrypoints_soundness; auto.
+          apply G_is_well_formed.
         * apply PS.maps_match_on_reflexive.
-    - exists (PS.CC (PS.to_partial_stack s split, mem, Pointer.component pc)
-               PS.Normal).
+    - exists (PS.CC (PS.to_partial_stack s split, mem, Pointer.component pc) PS.Normal).
       split.
       + unfold PS.initial_state.
         subst. repeat split. auto.
+        * admit. (* TODO prove that program components have a memory *)
       + apply ContextControl_Normal; auto.
-        * unfold PS.is_context_component.
-          unfold PS.is_program_component.
-          subst mainC. rewrite Hpc_comp.
-          auto.
+        * unfold PS.is_context_component, PS.is_program_component.
+          subst mainC. auto.
+        * (* TODO prove that p's main component is in the interface *)
+          admit.
         * apply PS.maps_match_on_reflexive.
   Admitted.
 
@@ -92,10 +127,55 @@ Section Decomposition.
     inversion Hs1s2_rel; subst.
     - unfold executing. eexists. eexists. eauto.
       repeat split; eauto.
-      + (* TODO prove linking doesn't create problems *)
+      + unfold G, G'.
+        (* TODO prove that if G has a procedure, then G' has it as well *)
         admit.
     - reflexivity.
-    - admit.
+    - exfalso.
+      apply H9. intro. unfold CS.final_state.
+      unfold executing. eexists. eexists. eauto.
+  Admitted.
+
+  Lemma split_agrees_with_global_env:
+    forall C, PS.is_program_component G C -> In C split.
+  Proof.
+    intros C Hprog.
+    unfold PS.is_program_component, split in *.
+
+    assert (Hprogcomp := Hprog).
+    apply (wfgenv_entrypoints_soundness G G_is_well_formed) in Hprog.
+    unfold G in Hprog. unfold init_genv in Hprog.
+    destruct (init_all (program_link p c mainC mainP)).
+    simpl in Hprog. destruct p0. simpl in Hprog.
+    apply NMapExtra.update_in_iff in Hprog.
+    destruct Hprog.
+    - assert (H' := H).
+      apply NMapExtra.F.elements_in_iff in H'.
+      destruct H' as [CI Hin].
+      change C with (fst (C, CI)).
+      apply (in_map fst (NMap.elements (prog_interface p))).
+      (* TODO prove that InA => In *)
+      admit.
+    - admit. (* contradiction, the component belongs to the program *)
+  Admitted.
+
+  Lemma genv_extension_after_partialize_1:
+    forall C CI,
+      NMap.MapsTo C CI (genv_interface G') -> NMap.MapsTo C CI (genv_interface G).
+  Proof.
+  Admitted.
+
+  Lemma genv_extension_after_partialize_2:
+    forall C Cprocs,
+      NMap.MapsTo C Cprocs (genv_procedures G') -> NMap.MapsTo C Cprocs (genv_procedures G).
+  Proof.
+  Admitted.
+
+  Lemma genv_extension_after_partialize_3:
+    forall C Centrypoints,
+      NMap.MapsTo C Centrypoints (genv_entrypoints G') ->
+      NMap.MapsTo C Centrypoints (genv_entrypoints G).
+  Proof.
   Admitted.
 
   Lemma lockstep_simulation:
@@ -108,7 +188,11 @@ Section Decomposition.
   Proof.
     intros s1 t s1' Hstep s2 Hs1s2_rel.
     inversion Hs1s2_rel; subst;
-      inversion Hstep; subst.
+      inversion Hstep; subst;
+
+    (* extract the current component's memory *)
+    destruct H1 as [cmem Hcmem].
+
     (* the program has control and doesn't produce an event *)
     - admit.
     - admit.
@@ -124,31 +208,203 @@ Section Decomposition.
     - admit.
 
     (* the program has control and produces an event *)
-    - admit.
-    - admit.
+    - destruct (NMapExtra.F.In_dec (genv_entrypoints G) C') as [Htarget|Htarget].
+      (* internal call *)
+      + eexists. split.
+        * eapply PS.Program_Internal_Call; eauto.
+          ** admit.
+          ** admit.
+          ** unfold PS.is_program_component.
+             (* TODO prove that partialize preserves entrypoints (genv_extension) *)
+             admit.
+          ** admit.
+        * apply ProgramControl; auto.
+          ** (* TODO rethink this part *)
+             admit.
+          ** admit.
+      (* external call *)
+      + eexists. split.
+        * eapply PS.Program_External_Call; eauto.
+          ** admit.
+          ** admit.
+          ** unfold PS.is_program_component.
+             (* TODO prove that partialize preserves entrypoints (genv_extension) *)
+             admit.
+        * apply ContextControl_Normal.
+          ** admit.
+          ** admit.
+          ** admit.
+          ** auto.
+    - destruct (NMapExtra.F.In_dec (genv_entrypoints G) (Pointer.component pc'))
+                 as [Htarget|Htarget].
+      (* internal return *)
+      + eexists. split.
+        * eapply PS.Program_Internal_Return; auto.
+          ** admit.
+          ** (* TODO rethink this part *)
+            admit.
+          ** unfold PS.is_program_component.
+             (* TODO prove that partialize preserves entrypoints (genv_extension) *)
+             admit.
+        * apply ProgramControl; auto.
+          admit.
+      (* external return *)
+      + eexists. split.
+        * eapply PS.Program_External_Return; auto.
+          ** admit.
+          ** (* TODO partialize & context components *) admit.
+          ** (* TOOD rethink this part *) admit.
+        * apply ContextControl_Normal; auto.
+          admit.
 
     (* the context has control and doesn't produce an event *)
-    - admit.
-    - admit.
-    - admit.
-    - admit.
-    - admit.
-    - admit.
-    - admit.
-    - admit.
-    - admit.
-    - admit.
-    - admit.
-    - admit.
+    - eexists. split.
+      + apply PS.Context_Epsilon.
+      + assert (Hpc: Pointer.component pc = Pointer.component (Pointer.inc pc)). {
+          destruct pc. destruct p0. reflexivity.
+        } rewrite Hpc.
+        apply ContextControl_Normal with (pc:=Pointer.inc pc).
+        * rewrite <- Hpc. auto.
+        * reflexivity.
+        * rewrite Pointer.inc_preserves_component.
+          eexists. eauto.
+        * auto.
+    - eexists. split.
+      + apply PS.Context_Epsilon.
+      + assert (Hpc: Pointer.component pc = Pointer.component (Pointer.inc pc)). {
+          destruct pc. destruct p0. reflexivity.
+        } rewrite Hpc.
+        apply ContextControl_Normal with (pc:=Pointer.inc pc).
+        * rewrite <- Hpc. auto.
+        * reflexivity.
+        * rewrite Pointer.inc_preserves_component.
+          eexists. eauto.
+        * auto.
+    - eexists. split.
+      + apply PS.Context_Epsilon.
+      + assert (Hpc: Pointer.component pc = Pointer.component (Pointer.inc pc)). {
+          destruct pc. destruct p0. reflexivity.
+        } rewrite Hpc.
+        apply ContextControl_Normal with (pc:=Pointer.inc pc).
+        * rewrite <- Hpc. auto.
+        * reflexivity.
+        * rewrite Pointer.inc_preserves_component.
+          eexists. eauto.
+        * auto.
+    - eexists. split.
+      + apply PS.Context_Epsilon.
+      + assert (Hpc: Pointer.component pc = Pointer.component (Pointer.inc pc)). {
+          destruct pc. destruct p0. reflexivity.
+        } rewrite Hpc.
+        apply ContextControl_Normal with (pc:=Pointer.inc pc).
+        * rewrite <- Hpc. auto.
+        * reflexivity.
+        * rewrite Pointer.inc_preserves_component.
+          eexists. eauto.
+        * auto.
+    - eexists. split.
+      + apply PS.Context_Epsilon.
+      + assert (Hpc: Pointer.component pc = Pointer.component (Pointer.inc pc)). {
+          destruct pc. destruct p0. reflexivity.
+        } rewrite Hpc.
+        apply ContextControl_Normal with (pc:=Pointer.inc pc).
+        * rewrite <- Hpc. auto.
+        * reflexivity.
+        * rewrite Pointer.inc_preserves_component.
+          eexists. eauto.
+        * auto.
+    - eexists. split.
+      + apply PS.Context_Epsilon.
+      + assert (Hpc: Pointer.component pc = Pointer.component (Pointer.inc pc)). {
+          destruct pc. destruct p0. reflexivity.
+        } rewrite Hpc.
+        apply ContextControl_Normal with (pc:=Pointer.inc pc).
+        * rewrite <- Hpc. auto.
+        * reflexivity.
+        * rewrite Pointer.inc_preserves_component.
+          eexists. eauto.
+        * auto.
+    - eexists. split.
+      + apply PS.Context_Epsilon.
+      + assert (Hpc: Pointer.component pc = Pointer.component (Pointer.inc pc)). {
+          destruct pc. destruct p0. reflexivity.
+        } rewrite Hpc.
+        apply ContextControl_Normal with (pc:=Pointer.inc pc).
+        * rewrite <- Hpc. auto.
+        * reflexivity.
+        * rewrite Pointer.inc_preserves_component.
+          admit.
+        * (* TODO prove that Memory.store preserves maps_match_on *)
+          admit.
+    - eexists. split.
+      + apply PS.Context_Epsilon.
+      + (* TODO prove that when using find_label_in_component we remain in the
+           same component *)
+        admit.
+    - eexists. split.
+      + apply PS.Context_Epsilon.
+      + rewrite <- H10. apply ContextControl_Normal; auto.
+        * rewrite H10. auto.
+        * rewrite H10. eexists. eauto.
+    - eexists. split.
+      + apply PS.Context_Epsilon.
+      + (* TODO prove that when using find_label_in_procedure we remain in the
+           same component *)
+        admit.
+    - eexists. split.
+      + apply PS.Context_Epsilon.
+      + assert (Hpc: Pointer.component pc = Pointer.component (Pointer.inc pc)). {
+          destruct pc. destruct p0. reflexivity.
+        } rewrite Hpc.
+        apply ContextControl_Normal; auto.
+        * rewrite <- Hpc. auto.
+        * rewrite Pointer.inc_preserves_component.
+          eexists. eauto.
+    - eexists. split.
+      + apply PS.Context_Epsilon.
+      + assert (Hpc: Pointer.component pc = Pointer.component (Pointer.inc pc)). {
+          destruct pc. destruct p0. reflexivity.
+        } rewrite Hpc.
+        apply ContextControl_Normal with (pc:=Pointer.inc pc).
+        * rewrite <- Hpc. auto.
+        * reflexivity.
+        * (* TODO prove that Memory.alloc preserves maps_match_on *)
+          admit.
+        * admit. (* TODO investigate more here *)
 
     (* the context has control and produces an event *)
-    - admit.
-    - admit.
+    - destruct (NMapExtra.F.In_dec (genv_entrypoints G) C') as [Htarget|Htarget].
+      (* internal call *)
+      + admit.
+      (* external call *)
+      + admit.
+    - destruct (NMapExtra.F.In_dec (genv_entrypoints G) (Pointer.component pc))
+        as [Htarget|Htarget].
+      (* internal return *)
+      + admit.
+      (* external return *)
+      + admit.
+
+    (* the context goes wrong *)
+    - exfalso. eapply H3. eauto.
+    - exfalso. eapply H3. eauto.
+    - exfalso. eapply H3. eauto.
+    - exfalso. eapply H3. eauto.
+    - exfalso. eapply H3. eauto.
+    - exfalso. eapply H3. eauto.
+    - exfalso. eapply H3. eauto.
+    - exfalso. eapply H3. eauto.
+    - exfalso. eapply H3. eauto.
+    - exfalso. eapply H3. eauto.
+    - exfalso. eapply H3. eauto.
+    - exfalso. eapply H3. eauto.
+    - exfalso. eapply H3. eauto.
+    - exfalso. eapply H3. eauto.
   Admitted.
 
   Theorem PS_simulates_CS:
-    forward_simulation (CS.sem (program_link p c (prog_main p)))
-                       (PS.sem p (prog_interface c)).
+    forward_simulation (CS.sem (program_link p c mainC mainP))
+                       (PS.sem p mainC mainP (prog_interface c)).
   Proof.
     apply forward_simulation_step with related_states.
     - apply initial_states_match.
@@ -158,9 +414,10 @@ Section Decomposition.
 
   Corollary PS_improves_CS_behavior:
     forall beh1,
-      program_behaves (CS.sem (program_link p c (prog_main p))) beh1 ->
+      program_behaves (CS.sem (program_link p c mainC mainP)) beh1 ->
     exists beh2,
-      program_behaves (PS.sem p (prog_interface c)) beh2 /\ behavior_improves beh1 beh2.
+      program_behaves (PS.sem p mainC mainP (prog_interface c)) beh2 /\
+      behavior_improves beh1 beh2.
   Proof.
     intros.
     eapply forward_simulation_behavior_improves; eauto.
@@ -169,8 +426,8 @@ Section Decomposition.
 
   Corollary PS_behaves_as_CS:
     forall beh,
-      program_behaves (CS.sem (program_link p c (prog_main p))) beh ->
-      program_behaves (PS.sem p (prog_interface c)) beh.
+      program_behaves (CS.sem (program_link p c mainC mainP)) beh ->
+      program_behaves (PS.sem p mainC mainP (prog_interface c)) beh.
   Proof.
   Admitted.
 End Decomposition.
